Sketch of Step 6

ntor/Games.ec
@@ -462,5 +462,312 @@ module Game4 = Game3 with {
 
 }.
 
+module Game5 : GAKE_out_i = {
+  var hm : (pkey * pkey * s_id * pkey * pkey, tag * key) fmap
+
+  var servers : (s_id, server_state) fmap
+
+  var c_smap : (int, pr_st_client instance_state) fmap
+  var s_smap : (s_id * int, pr_st_server instance_state) fmap
+  
+  var tested : bool
+  
+  var kp_set : ((pkey * skey)) fset
+  var bad : bool
+
+
+  proc init_mem() : unit = {
+    hm <- empty;
+    servers <- empty;
+    c_smap <- empty;
+    s_smap <- empty;
+    tested <- false;
+    kp_set <- fset0;
+    bad <- false;
+  }
+  
+  (* random oracle *)
+  proc h(x: pkey * pkey * s_id * pkey * pkey) : tag * key = {
+    var tk;
+
+    tk <$ dtag `*` dkey;
+    if (x \notin hm) {
+      hm.[x] <- tk;
+    }
+    
+    return oget hm.[x];
+  }
+
+  (* server management *)
+  proc init_s(b: s_id) : pkey option = {
+    var kp;
+
+    if (b \notin servers) {
+      kp <$ dkp;
+      bad <- bad \/ kp \in kp_set;
+      if (!bad) {
+        kp_set <- kp_set `|` fset1 kp;
+        servers.[b] <- Honest kp;
+      }
+    }
+    return omap get_pkey servers.[b];
+  }
+  
+  proc set_cert(b: s_id, pk: pkey) : unit option = {
+    var r <- None;
+
+    if (b \notin servers) {
+      servers.[b] <- Dishonest pk;
+      r <- Some ();
+    }
+    return r;
+  }
+
+  proc send_msg1(i: int, m1: s_id) : pkey option = {
+    var st, pk_b, kp;
+    var r <- None;
+
+    st <- c_smap.[i];
+    if (m1 \in servers) {
+      pk_b <- get_pkey (oget servers.[m1]);
+      match st with
+      | None => {
+          kp <$ dkp;
+          bad <- bad \/ kp \in kp_set;
+          if (!bad) {
+            kp_set <- kp_set `|` fset1 kp;
+            c_smap.[i] <- Pending (m1, pk_b, fst kp, snd kp) (fst kp) (false, false, false);
+            r <- Some (fst kp);
+          }
+        }
+      | Some st => {
+          match st with
+          | Pending st pt ir => c_smap.[i] <- Aborted (Some st) (Some (pt, None)) ir;
+          | Accepted _ _ _ _ => { }
+          | Aborted _ _ _ => { }
+          end;
+        }
+      end;
+    }
+    return r;
+  }
+
+  proc send_msg2(b: s_id, j: int, m2: pkey) : (pkey * tag) option = {
+    var sko, kp, t_B, sk;
+    var r <- None;
+
+    sko <- obind get_skey servers.[b];
+    if (sko is Some sk_b) (* Server was initialised as honest *) {
+      match s_smap.[b, j] with
+      | None => {
+          kp <$ dkp;
+          bad <- bad \/ kp \in kp_set;
+          if (!bad) {
+            kp_set <- kp_set `|` fset1 kp;
+            (t_B, sk) <@ h(m2 ^ kp.`2, m2 ^ sk_b, b, m2, kp.`1);
+            s_smap.[(b, j)] <- Accepted (b, sk_b, Some kp.`2) (m2, Some (kp.`1, t_B)) sk (false, false, false);
+            r <- Some (kp.`1, t_B);
+          }
+        }
+      | Some st => { (* only completed sessions would be stored, and those can't be aborted; do nothing *) }
+      end;
+    }
+
+    return r;
+  }
+
+  proc send_msg3(i: int, m3: pkey * tag) : unit option = {
+    var b, pk_b, pk_ce, sk_ce, t_A, sk;
+    var r <- None;
+
+    match c_smap.[i] with
+    | None => { } (* Abort? *)
+    | Some _ => {
+        match oget c_smap.[i] with
+        | Pending st pt ir => {
+            (b, pk_b, pk_ce, sk_ce) <- st;
+            (t_A, sk) <@ h(m3.`1 ^ sk_ce, pk_b ^ sk_ce, b, pk_ce, m3.`1);
+            if (t_A = m3.`2) {
+              c_smap.[i] <- Accepted st (pt, Some m3) sk ir;
+              r <- Some ();
+            } else {
+              c_smap.[i] <- Aborted (Some st) (Some (pt, Some m3)) ir;
+            }
+          }
+        | Accepted _ _ _ _ => { }
+        | Aborted _ _ _ => { }
+        end;
+      }
+    end;
+    return r;
+  }
+
+
+(* reveal and test *)
+  proc c_rev_skey(i: int) : key option = {
+    var k <- None;
+
+    match c_smap.[i] with
+    | None => { }
+    | Some _ => {
+        (* only accepted client instances that are not tested and 
+           that not only have tested partners can be sesskey revealed *)
+        if (oget c_smap.[i] is Accepted st' t' k' ir') {
+          if (!(get_ir_test (oget c_smap.[i]) \/ untested_partner_c t' s_smap = Some false)) {
+            k <- Some k';
+            c_smap.[i] <- set_ir_sess (Accepted st' t' (oget k) ir');
+          }
+        }
+      }
+    end;
+    return k;
+  }
+
+  proc s_rev_skey(b: s_id, j: int) : key option = {
+    var k <- None;
+
+    match s_smap.[(b, j)] with
+    | None => { }
+    | Some _ => {
+        (* only accepted server instances that are not tested and 
+           that not only have tested partners can be sesskey revealed *)
+        if (oget s_smap.[b, j] is Accepted st' t' k' ir') {
+          if (!(get_ir_test (oget s_smap.[b, j]) \/ untested_partner_s t' c_smap = Some false)) {
+            k <- Some k';
+            s_smap.[(b, j)] <- set_ir_sess (Accepted st' t' (oget k) ir');
+          }
+        }
+      }
+    end;
+    return k;
+  }
+
+  proc rev_ltkey(b: s_id) : skey option = {
+    var ltk <- None;
+
+    match servers.[b] with
+    | None => { }
+    | Some _ => {
+        (* a server can be ltkey revealed if no instance of it is ephkey revealed 
+           in case that instance or all its partners are tested *) 
+        if (oget servers.[b] is Honest kp) {
+          if (forall j,
+                (b, j) \in s_smap (* just checking instances of b *)
+                => !(   (   get_ir_test (oget s_smap.[b, j])
+                            (* This is always OK (get_trace always Some on server side *)
+                         \/ untested_partner_s (oget (get_trace (oget s_smap.[b, j]))) c_smap = Some false)
+                     /\ get_ir_eph (oget s_smap.[b,j]))) {
+            ltk <- Some kp.`2; 
+            servers.[b] <- Corrupt kp; 
+          }
+        }
+      }
+    end;
+    return ltk;
+  }
+
+  proc c_rev_ephkey(i: int) : skey option = {
+    var ek <- None;
+
+    match c_smap.[i] with
+    | None => { }
+    | Some _ => {
+        match oget c_smap.[i] with
+          (* client instances can be ephkey revealed when pending if there isn't 
+             a tested origin partner (agreeing on first message *)
+        | Pending st pk_e ir => {
+            if (untested_origins_c (pk_e, None) s_smap <> Some false) {
+              ek <- Some (get_eph_c st);
+              c_smap.[i] <- set_ir_eph (Pending st pk_e ir);
+            }
+          }
+          (* accepted client instamces can only be ephkey revealed when not tested and 
+             if not all partners are tested *)
+        | Accepted st t k ir => {
+            if (!(get_ir_test (oget c_smap.[i]) \/ untested_partner_c t s_smap = Some false)) {
+              ek <- Some (get_eph_c st);
+              c_smap.[i] <- set_ir_eph (Accepted st t k ir);
+            }
+          }
+        | Aborted _ _ _ => {  }
+        end;
+      }
+    end;
+    return ek;
+  }
+
+  proc s_rev_ephkey(b: s_id, j: int) : skey option = {
+    var ek <- None;
+
+    match s_smap.[b, j] with
+    | None => { }
+    | Some _ => {
+        (* only accepted server instances that are not ltkey revealed in case they 
+           or all partners are tested can be ephkey revealed *)
+        if (oget s_smap.[b, j] is Accepted st t k ir) { (* No Pending on Server side *)
+          if (!((   get_ir_test (oget s_smap.[b, j])
+                 \/ untested_partner_s t c_smap = Some false)
+                /\ get_sr_ltk (oget servers.[b]))) {
+            ek <- Some (get_eph_s st);
+            s_smap.[(b, j)] <- set_ir_eph (Accepted st t k ir);
+          }
+        }
+      }
+    end;
+    return ek;
+  }
+
+  proc c_test(i: int) : key option = {
+    var k <- None;
+    var ks;
+
+    if (!tested) {
+      match c_smap.[i] with
+      | None => { }
+      | Some _ => {
+          (* only accepted client instances that are not sesskey revealed, not ephkey revealed 
+             and not all partner instances are unfresh can be tested *)
+          if (oget c_smap.[i] is Accepted st' t' k' ir') {
+            if (!(   get_ir_sess (oget c_smap.[i]) \/ get_ir_eph (oget c_smap.[i]) 
+                  \/ fresh_partner_c t' s_smap servers = Some false)) {
+              ks <$ dkey;
+              k <- Some ks;
+              c_smap.[i] <- set_ir_test (Accepted st' t' ks ir');
+              tested <- true;
+            }
+          }
+        }
+      end;
+    }
+    return k;
+  }
+
+  proc s_test(b: s_id, j: int) : key option = {
+    var k <- None;
+    var ks;
+
+    if (!tested) {
+      match s_smap.[(b, j)] with
+      | None => { }
+      | Some _ => {
+          (* only accepted server instances that are not sesskey revealed, not trivially broken
+             and not all partner instances are unfresh can be tested *)
+          if (oget s_smap.[b, j] is Accepted st' t' k' ir') {
+            if (!(   get_ir_sess (oget s_smap.[b, j]) 
+                  \/ (get_ir_eph (oget s_smap.[b, j]) /\ get_sr_ltk (oget servers.[b]))
+                  \/ fresh_partner_s t' c_smap = Some false)) {
+              ks <$ dkey;
+              k <- Some ks;
+              s_smap.[(b, j)] <- set_ir_test (Accepted st' t' ks ir');
+              tested <- true;
+            }
+          }
+        }
+      end;
+    }
+    return k;
+  }
+}.
+
 
 print Game4.
